theories/lang/mailbox_extra.v
@@ -8,122 +8,61 @@ Context {HyperConst : HypervisorConstants}.
 Implicit Type σ : state.
 Implicit Type i : VMID.
 
-Lemma empty_rx_global_preserve_current_vm σ i :
-  get_current_vm (empty_rx_global σ i) = get_current_vm σ.
+Lemma empty_rx_preserve_current_vm σ :
+  get_current_vm (empty_rx σ) = get_current_vm σ.
 Proof.
-  rewrite /empty_rx_global.
-  rewrite (surjective_pairing (get_mail_box σ @ i)).
-  by rewrite (surjective_pairing (get_mail_box σ @ i).2).
+  rewrite /empty_rx.
+  destruct (σ.1.1.1.1.2 !!! σ.1.1.2).
+  destruct p.
+  done.
 Qed.
 
-Lemma empty_rx_global_preserve_mem σ i :
-  get_mem (empty_rx_global σ i) = get_mem σ.
+Lemma empty_rx_preserve_mem σ:
+  get_mem (empty_rx σ) = get_mem σ.
 Proof.
-  rewrite /empty_rx_global.
-  rewrite (surjective_pairing (get_mail_box σ @ i)).
-  by rewrite (surjective_pairing (get_mail_box σ @ i).2).
+  rewrite /empty_rx.
+  destruct (σ.1.1.1.1.2 !!! σ.1.1.2).
+  destruct p.
+  done.
 Qed.
 
-Lemma empty_rx_global_preserve_regs σ i :
- get_reg_gmap (empty_rx_global σ i) = get_reg_gmap σ.
+Lemma empty_rx_preserve_regs σ:
+ get_reg_gmap (empty_rx σ) = get_reg_gmap σ.
 Proof.
-  rewrite /empty_rx_global.
-  rewrite (surjective_pairing (get_mail_box σ @ i)).
-  by rewrite (surjective_pairing (get_mail_box σ @ i).2).
+  rewrite /empty_rx.
+  destruct (σ.1.1.1.1.2 !!! σ.1.1.2).
+  destruct p.
+  done.
 Qed.
 
-(* TODO *)
-Lemma empty_rx_global_preserve_mb σ i :
-  get_mb_gmap (empty_rx_global σ i) = (get_mb_gmap σ).
+Lemma empty_rx_preserve_mb σ:
+  get_mb_gmap (empty_rx σ) = (get_mb_gmap σ).
 Proof.
-  rewrite /empty_rx_global.
-  rewrite (surjective_pairing (get_mail_box σ @ i)).
-  rewrite (surjective_pairing (get_mail_box σ @ i).2).
-  rewrite /get_mb_gmap /=.
-  f_equal.
-  (* apply (list_eq_same_length _ _ (2*vm_count)). *)
-  (* induction list_of_vmids eqn:Heqn. *)
-  (* { assert (length list_of_vmids = 0). *)
-  (*   { rewrite Heqn. done. } *)
-  (*   rewrite length_list_of_vmids in H. *)
-  (*   simpl. *)
-  (*   lia. *)
-  (*   } *)
-  (*   simpl. *)
+  rewrite /empty_rx.
 (* XXX: couldn't find useful lemmas about flat_map, maybe redefine get_mb_gmap? *)
 Admitted.
-(*   rewrite list_length. *)
-(*   rewrite fmap_length. *)
-(*   rewrite fmap_length. *)
-(*   apply length_list_of_vmids. *)
-(*   intros. *)
-(*   apply list_lookup_fmap_inv in H0, H1. *)
-(*   destruct H0, H1. *)
-(*   destruct H0, H1. *)
-(*   rewrite H3 in H2. *)
-(*   inversion H2;subst x1. *)
-(*   clear H2. *)
-(*   rewrite H0 H1. *)
-(*   do 2 f_equal. *)
-(*   rewrite /get_vm_mail_box /get_mail_boxes /=. *)
-(*   destruct (decide (i = x0)). *)
-(*   subst x0. *)
-(*   by rewrite vlookup_insert //. *)
-(*   by rewrite vlookup_insert_ne //. *)
-(* Qed. *)
 
-Lemma empty_rx_global_preserve_pagetable σ i:
-  get_page_table (empty_rx_global σ i)  = get_page_table σ.
+Lemma empty_rx_preserve_pagetable σ:
+  get_page_table (empty_rx σ)  = get_page_table σ.
 Proof.
-  rewrite /empty_rx_global.
-  rewrite (surjective_pairing (get_mail_box σ @ i)).
-  by rewrite (surjective_pairing (get_mail_box σ @ i).2).
+  rewrite /empty_rx.
+  destruct (σ.1.1.1.1.2 !!! σ.1.1.2).
+  destruct p.
+  done.
 Qed.
 
-Lemma empty_rx_global_preserve_owned σ i :
-  get_own_gmap (empty_rx_global σ i) = (get_own_gmap σ).
+Lemma empty_rx_preserve_trans σ :
+  get_transactions (empty_rx σ) = (get_transactions σ).
 Proof.
-  rewrite /empty_rx_global.
-  rewrite (surjective_pairing (get_mail_box σ @ i)).
-  by rewrite (surjective_pairing (get_mail_box σ @ i).2).
+  rewrite /empty_rx.
+  destruct (σ.1.1.1.1.2 !!! σ.1.1.2).
+  destruct p.
+  done.
 Qed.
-
-Lemma empty_rx_global_preserve_access σ i :
-  get_access_gmap (empty_rx_global σ i) = (get_access_gmap σ).
-Proof.
-  rewrite /empty_rx_global.
-  rewrite (surjective_pairing (get_mail_box σ @ i)).
-  by rewrite (surjective_pairing (get_mail_box σ @ i).2).
-Qed.
-
-Lemma empty_rx_global_preserve_trans σ i :
-  get_trans_gmap (empty_rx_global σ i) = (get_trans_gmap σ).
-Proof.
-  rewrite /empty_rx_global.
-  rewrite (surjective_pairing (get_mail_box σ @ i)).
-  by rewrite (surjective_pairing (get_mail_box σ @ i).2).
-Qed.
-
-Lemma empty_rx_global_preserve_trans' σ i :
-  get_transactions (empty_rx_global σ i) = (get_transactions σ).
-Proof.
-  rewrite /empty_rx_global.
-  rewrite (surjective_pairing (get_mail_box σ @ i)).
-  by rewrite (surjective_pairing (get_mail_box σ @ i).2).
-Qed.
-
-Lemma empty_rx_global_preserve_retri σ i :
-  get_retri_gmap (empty_rx_global σ i) = (get_retri_gmap σ).
-Proof.
-  rewrite /empty_rx_global.
-  rewrite (surjective_pairing (get_mail_box σ @ i)).
-  by rewrite (surjective_pairing (get_mail_box σ @ i).2).
-Qed.
-
 
 (* TODO simplify *)
-Lemma empty_rx_global_update_mailbox σ l :
-  get_rx_gmap (empty_rx_global σ l) = <[l := None]>(get_rx_gmap σ).
+Lemma empty_rx_update_mailbox σ:
+  get_rx_gmap (empty_rx σ) = <[(get_current_vm σ) := None]>(get_rx_gmap σ).
 Proof.
   rewrite /get_rx_gmap.
   apply map_eq.
@@ -131,7 +70,7 @@ Proof.
   destruct (list_to_map
     (map
        (λ v : VMID,
-          match get_transactions (get_transactions get_mail_boxes empty_rx_global σ l !!! v) with
+          match get_transactions (get_transactions get_mail_boxes empty_rx σ !!! v) with
           | Some (l0, j) => (v, Some (l0, j))
           | None => (v, None)
           end) list_of_vmids) !! i) eqn:Heqn.
@@ -140,11 +79,11 @@ Proof.
     apply in_map_iff in Heqn.
     destruct Heqn as [y [Heqn1 Heqn2]].
     apply elem_of_list_In in Heqn2.
-    rewrite /empty_rx_global //= in Heqn1.
-    rewrite (surjective_pairing (get_mail_box σ @ l)) in Heqn1.
-    rewrite (surjective_pairing (get_mail_box σ @ l).2) in Heqn1.
+    rewrite /empty_rx //= in Heqn1.
+    destruct (σ.1.1.1.1.2 !!! σ.1.1.2).
+    destruct p.
     simpl in Heqn1.
-    destruct (decide (l = y)).
+    destruct (decide ((get_current_vm σ) = y)).
     + subst.
       rewrite vlookup_insert in Heqn1.
       simpl in Heqn1.
@@ -211,11 +150,11 @@ Proof.
            split; auto.
   - symmetry.
     rewrite <-not_elem_of_list_to_map in Heqn.
-    rewrite /empty_rx_global //= in Heqn.
-    rewrite (surjective_pairing (get_mail_box σ @ l)) in Heqn.
-    rewrite (surjective_pairing (get_mail_box σ @ l).2) in Heqn.
+    rewrite /empty_rx //= in Heqn.
+    destruct (σ.1.1.1.1.2 !!! σ.1.1.2).
+    destruct p.
     simpl in Heqn.
-    destruct (decide (l = i)).
+    destruct (decide ((get_current_vm σ) = i)).
     + subst.
       exfalso.
       apply Heqn.
@@ -224,7 +163,7 @@ Proof.
       rewrite /fill_rx_unsafe //=.
       apply elem_of_list_In.
       apply in_map_iff.
-      exists i.
+      exists (get_current_vm σ).
       split; auto using in_list_of_vmids.
       rewrite vlookup_insert //=.
     + rewrite /fill_rx_unsafe //=.
@@ -266,17 +205,3 @@ Proof.
 Qed.
 
 End mailbox_extra.
-
-Ltac rewrite_empty_rx_global :=
-  match goal with
-  | |- _ =>
-    try rewrite -> empty_rx_global_preserve_current_vm;
-    try rewrite -> empty_rx_global_preserve_regs;
-    try rewrite -> empty_rx_global_preserve_mem;
-    try rewrite -> empty_rx_global_preserve_mb;
-    try rewrite -> empty_rx_global_preserve_owned;
-    try rewrite -> empty_rx_global_preserve_access;
-    try rewrite -> empty_rx_global_preserve_trans;
-    try rewrite -> empty_rx_global_preserve_trans';
-    try rewrite -> empty_rx_global_preserve_retri
-  end.
